src/proof/k8s_io/api/apps/v1_init.v
@@ -5,6 +5,13 @@ From New.proof.k8s_io.api.core Require Export v1_init.
 Section proof.
 Context `{hG: heapGS Σ} `{!ffi_semantics _ _} {go_ctx: GoContext}.
 
+(* TODO: carry the globals in IsPkgInit *)
+(* Definition is_initialized : iProp Σ :=
+  ∃ (gv: schema.GroupVersion.t),
+    "#HglobalSchemeGroupVersion" ∷ (global_addr v1.SchemeGroupVersion) ↦□ gv ∗
+    "%HSchemeGroupVersion_Group" ∷ ⌜ gv.(schema.GroupVersion.Group') = "apps"%go ⌝ ∗
+    "%HSchemeGroupVersion_Version" ∷ ⌜ gv.(schema.GroupVersion.Version') = "v1"%go ⌝. *)
+
 #[global] Instance : IsPkgInit code.k8s_io.api.apps.v1.v1 := define_is_pkg_init True%I.
 #[global] Instance : GetIsPkgInitWf code.k8s_io.api.apps.v1.v1 := build_get_is_pkg_init_wf.
 
